\documentclass{report} 
\title{Appendix 3}
\date{Started 5 Nov 2024}
\author{Malcolm}
\usepackage{amsmath} %import math
\usepackage{mathtools} %more math
\usepackage{amssymb} %for QED symbol
\usepackage{amsthm} %
\usepackage{bm}%bold math
\usepackage{graphicx} %import imaging
\graphicspath{{./images/}} %set imaging path
\begin{document}
\maketitle

\tableofcontents

\appendix
\chapter{Probability}

\section{Fundamental concepts}
\subsection{Expectation and Variance}
\textbf{Expectation}\\
We define the \textit{expected value} of a random variable $X$ with a PMF $p_X$ by
\begin{equation*}
\boxed{\mathbb{E}[X]=\sum_xxp_X(x)}
\end{equation*}
\textbf{Variance and Standard Deviation}\\
We define the \textit{variance} associated with a random variable $X$ as
\begin{equation*}
\boxed{\text{var}(X)=\mathbb{E}\left[(X-\mathbb{E}[X])^2\right]=\sum_x(X-\mathbb{E}[X])^2p_X(x)}
\end{equation*}
(See that the because of the square the variance is always nonnegative). The variance provides a measure of
dispersion of $X$ around the mean. Another measure of dispersion is the \textit{Standard deviation} of $X$, which 
is defined as the square root of the variance and is denoted by $\sigma_X$:
\begin{equation*}
\boxed{\sigma_X=\sqrt{\text{var}(X)}}
\end{equation*}
The standard deviation is often easier to interpret because it has the same units as $X$.
\newpage

\subsection{Expected value of a function of a RV}
\textbf{Expectation of a function}\\
Let $X$ be a RV with PMF $p_X$, and let $g(X)$ be a function of $X$. Then the expected value
of the random variable $g(X)$ is given by
\begin{equation*}
\boxed{\mathbb{E}[g(X)]=\sum_xg(x)p_X(x)}
\end{equation*}
This can be shown, since
\begin{equation*}
p_Y(y)=\sum_{\{x|g(x)=y\}}p_X(x)
\end{equation*}
we have
\begin{align*}
\mathbb{E}[g(X)]&=\mathbb{E}[Y]\\
&=\sum_yyp_Y(y)\\
&=\sum_yy\sum_{\{x|g(x)=y\}}p_X(x)\\
&=\sum_y\sum_{\{x|g(x)=y\}}yp_X(x)\\
&=\sum_y\sum_{\{x|g(x)=y\}}g(x)p_X(x)\\
&=\sum_xg(x)p_X(x)
\end{align*}
\textbf{Variance}\\
Using this we can write the variance of $X$ as
\begin{equation*}
\text{var}(X)=\mathbb{E}\left[(X-\mathbb{E}[X])^2\right]
=\sum_x(X-\mathbb{E}[X])^2p_X(x)
\end{equation*}
\newpage

\subsection{Expectation and variance of linear functions}
We show for a random variable $X$, and letting $Y=aX+b$:
\begin{equation*}
\boxed{\mathbb{E}[Y]=a\mathbb{E}[X]+b,\quad
\text{var}(Y)=a^2\text{var}(X)}
\end{equation*}
Linearity of Expectations:
\begin{equation*}
\mathbb{E}[Y]=\sum_x(ax+b)p_X(x)=a\underbrace{\sum_xxp_x(x)}_{=\mathbb{E}[X]}+b\underbrace{\sum_xp_x(x)}_{=1}
=a\mathbb{E}[X]+b
\end{equation*}
Variance:
\begin{align*}
\text{var}(Y)&=\sum_x(ax+b-\mathbb{E}[aX+b])^2p_X(x)\\
&=\sum_x(ax+b-a\mathbb{E}[X]+b)^2p_X(x)\\
&=a^2\sum_x(x-\mathbb{E}[X])^2p_X(x)\\
&=a^2\text{var}(X)
\end{align*}
Note that unless $g(X)$ is a linear function, it is not generally true that $\mathbb{E}[g(X)]$ is equal to 
$g(\mathbb{E}[X])$.

\subsection{Variance in terms of Moments Expression}
We show
\begin{equation*}
\boxed{\text{var}(X)=\mathbb{E}[X^2]-(\mathbb{E}[X])^2}
\end{equation*}
see that
\begin{align*}
\text{var}(X)&=\sum_x(x-\mathbb{E}[X])^2p_X(x)\\
&=\sum_x(x^2-2x\mathbb{E}[X]+(\mathbb{E}[X])^2)p_X(x)\\
&=\sum_xx^2p_X(x)-2\mathbb{E}[X]\sum_xxp_X(x)+(\mathbb{E}[X])^2\sum_xp_X(x)\\
&=\mathbb{E}[X^2]-2(\mathbb{E}[X])^2+(\mathbb{E}[X])^2\\
&=\mathbb{E}[X^2]-(\mathbb{E}[X])^2
\end{align*}
\newpage

\subsection{Expectation and Variance of Bernoulli}
Consider a Bernoulli RV $X$ with PMF
\begin{equation*}
p_X(k)=\begin{cases}
p,&\text{if }k=1.\\
1-p,&\text{if }k=0.
\end{cases}
\end{equation*}
The mean, second moment, and variance of $X$ are as follows:
\begin{align*}
\mathbb{E}[X]&=1\cdot p+0\cdot(1-p)=p\\
\mathbb{E}[X^2]&=1^2\cdot p+0\cdot(1-p)=p\\
\text{var}(X)&=\mathbb{E}[X^2]-(\mathbb{E}[X])^2
=p-p^2=p(1-p)
\end{align*}

\subsection{Expectation of Discrete Uniform}
Consider a Discrete Uniform RV $X$ with PMF, for $k\in[a,b]$:
\begin{equation*}
p_X(k)=\begin{cases}
\frac{1}{b-a+1},&\text{if }k=a,a+1\ldots,b\\
0,&\text{otherwise}.
\end{cases}
\end{equation*}
An illustration is useful here:
\begin{figure}[h]
\begin{center}
\includegraphics[width=10cm]{1}\\
\end{center}
\textbf{Expectation}\\
Upon inspection one might suppose that the expectation is
\begin{equation*}
\mathbb{E}[X]=\frac{a+b}{2}
\end{equation*}
\end{figure}\\
(next page)
\newpage
\noindent\textbf{Expectation (cont.)}\\
The formula can be elucidated from the definition of the expectation. First see that a sequence
$\sum^b_{k=a}k$ can be written as
\begin{align*}
\sum^b_{k=a}k&=\sum^b_{k=1}k-\sum^{a-1}_{k=1}k\\
&=\frac{(b)(b+1)}{2}-\frac{(a-1)(a)}{2}\quad\text{(see \ref{supnotes:1})}\\
&=\frac{b^2+b-a^2+a}{2}=\frac{(b-a+1)(a+b)}{2}
\end{align*}
The last step isn't easy to factor, but working back from our `hypothesis' for the expectation it coincides.\\
\vspace{1mm}\\
so now we have
\begin{align*}
\mathbb{E}[X]&=\sum^b_{k=a}k\left(\frac{1}{b-a+1}\right)\\
&=\frac{1}{b-a+1}\sum^b_{k=a}k\\
&=\frac{1}{b-a+1}\cdot\frac{(b-a+1)(a+b)}{2}\\
\mathbb{E}[X]&=\frac{(a+b)}{2}
\end{align*}
\newpage

\subsection{Variance of Discrete Uniform}
\textbf{Case for $k\in[1,n]$}:\\
We can obtain the second moment for a discrete uniform distributed over $k\in[1,n]$ as
\begin{align*}
\mathbb{E}[X^2]&=\sum^{n}_{k=1}k^2\left(\frac{1}{n}\right)\\
&=\frac{1}{n}\sum^{n}_{k=1}k^2\\
&=\frac{1}{n}\cdot\frac{n(n+1)(2n+1)}{6}\quad\text{(see \ref{supnotes:4})}\\
&=\frac{(n+1)(2n+1)}{6}
\end{align*}
We then use the formula for variance in terms of moments expression:
\begin{align*}
\text{var}(X)&=\mathbb{E}[X^2]-(\mathbb{E}[X])^2\\
&=\frac{(n+1)(2n+1)}{6}-\left(\frac{n+1}{2}\right)^2\\
&=\frac{1}{12}(n+1)(4n+2-3n-3)\\
&=\frac{n^2-1}{12}
\end{align*}
\textbf{General case} $k\in[a,b]$:\\
For the general case, note that a RV uniformly distributed over an interval $[a,b]$ has the \textit{same variance}
as one which is uniformly distributed over $[1,b-a+1]$---the PMF of the second is just a shifted version
of the PMF of the first.\\
\vspace{1mm}\\
Therefore, the desired variance is given by the first case, but instead with $n=b-a+1$, yielding
\begin{equation*}
\boxed{\text{var}(X)=\frac{(b-a+1)^2-1}{12}=\frac{(b-a)(b-a+2)}{12}}
\end{equation*}

\subsection{}




\chapter{Supplementary Notes}

\section{The sum of the first $n$ natural numbers is $n(n+1)/2$}
\label{supnotes:1}
We have that
\begin{equation*}
\sum^i_{i=1}i=1+2+\cdots+n
\end{equation*}
Now consider $2\sum^n_{i=1}i$:
\begin{align*}
2\sum^n_{i=1}i&=2(1+2+\cdots+(n-1)+n)\\
&=(1+2+\cdots+(n-1)+n)+(n+(n-1)+\cdots+2+1)\\
&=(1+n)+(2+(n-1))+\cdots+((n-1)+2)+(n+1)\\
&=(n+1)_1+(n+1)_2+\cdots+(n+1)_n\\
&=n(n+1)
\end{align*}
so
\begin{align*}
2\sum^n_{i=1}i&=n(n+1)\\
\sum^n_{i=1}i&=\frac{n(n+1)}{2}
\end{align*}
\newpage

\section{Telescoping series}
\label{supnotes:2}
Let $\langle b_n\rangle$ be a sequence in $\mathbb{R}$. Let $\langle a_n\rangle$ be a sequence defined as
\begin{equation*}
a_k=b_k-b_{k-1}
\end{equation*}
we show
\begin{equation*}
\boxed{\sum^n_{k=m}a_k=b_n-b_{m-1}}
\end{equation*}
See that
\begin{align*}
\sum^n_{k=m}a_k&=\sum^n_{k=m}(b_k-b_{k-1})\\
&=\sum^n_{k=m}b_k-\sum^n_{k=m}b_{k-1}\\
&=\sum^n_{k=m}b_k-\sum^{n-1}_{k=m-1}b_k\\
&=\left(\sum^{n-1}_{k=m}b_k+b_n\right)-\left(b_{m-1}+\sum^{n-1}_{k=m}b_k\right)\\
&=b_n-b_{m-1}
\end{align*}
\newpage

\section{Sum of series of products of consecutive integers}
\label{supnotes:3}
We show
\begin{align*}
\boxed{\sum^n_{j=1}j(j+1)=1\cdot2+2\cdot3+\cdots
+n(n+1)=\frac{n(n+1)(n+2)}{3}}
\end{align*}
See that
\begin{align*}
3i(i+1)&=i(i+1)(i+2)-i(i+1)(i-1)\\
&=(i+1)((i+1)+1)((i+1)-1)-i(i+1)(i-1)
\end{align*}
Thus we have the basis of a telescoping series (see (\ref{supnotes:2})):
\begin{equation*}
3i(i+1)=b(i+1)-b(i)
\end{equation*}
where
\begin{equation*}
b(i)=i(i+1)(i-1)
\end{equation*}
So we have
\begin{align*}
\sum^n_{j=1}3j(j+1)&=\sum^n_{j=1}(j+1)((j+1)+1)((j+1)-1)-j(j+1)(j-1)\\
&=n(n+1)(n+2)-0(0+1)(0-1)\\
&=n(n+1)(n+2)
\end{align*}
Thus
\begin{equation*}
\sum^n_{j=1}j(j+1)=\frac{n(n+1)(n+2)}{3}
\end{equation*}
\newpage

\section{Sum of sequence of squares}
\label{supnotes:4}
We show
\begin{equation*}
\boxed{\forall n\in\mathbb{N}:
\sum^n_{i=1}i^2=\frac{n(n+1)(2n+1)}{6}}
\end{equation*}
See that this follows from (\ref{supnotes:3}):
\begin{align*}
\sum^n_{i=1}3i(i+1)&=n(n+1)(n+2)\\
\sum^n_{i=1}3i^2+\sum^n_{i=1}3i&=n(n+1)(n+2)\\
\sum^n_{i=1}3i^2&=n(n+1)(n+2)-3\frac{n(n+1)}{2}\quad\text{see (\ref{supnotes:1}))}\\
\sum^n_{i=1}i^2&=\frac{n(n+1)(n+2)}{3}-\frac{n(n+1)}{2}\\
&=\frac{2n(n+1)(n+2)-3n(n+1)}{6}\\
&=\frac{n(n+1)(2n+1)}{6}
\end{align*}














\end{document}
